Start changing the type path to be path_t.
path_t is the type of non-empty sequences of blocks, instead of just sequences of blocks.
The representation is inspired by ssreflect.path. The question of whether we should
directly use ssreflect.path is still unclear. My intuition is that we don't want to use
it because there (in ssreflect.path), path is defined merely as a boolean predicate.
Moreover, there is not lots of support for uniq---support for uniq would have been
the main appeal of using an existing path representation.

Common/Memory.v
@@ -276,7 +276,53 @@ Module Memory.
     | Some compMem => ComponentMemory.load_block compMem (snd pair)
     end.
 
+  
+
   (* Have path be the type of non-empty sequences? *)
+  Definition node_t : Type := Component.id * Block.id.
+
+  (* Taking inspiration from mathcomp.ssreflect.path, make path be the type of
+     non-empty sequences.
+     A path is thus a head and a tail. The head is of type node_t, and the tail of type
+     seq node_t.
+     Our path is also uniq, i.e., no cycles.
+   *)
+  Definition path_t : Type := node_t * (seq node_t).
+  Definition uniq_path_t (p : path_t) : bool := uniq (p.1 :: p.2).
+
+  Definition extend_path' (m : t) (p : path_t) : list path_t :=
+    map (fun x => (x, p.1 :: p.2))
+        (filter (fun x => (x \notin p.2) && (x != p.1)) (apply_load_block m p.1)).
+
+  Lemma extend_path'_returns_extensions :
+    forall m p0 ps,
+      extend_path' m p0 = ps -> all (fun p => (p.2 == p0.1 :: p0.2)) ps.
+  Proof.
+    intros. subst ps. unfold extend_path'.
+    rewrite all_map. simpl.
+    unfold preim. simpl.
+    rewrite eq_refl.
+    apply all_predT.
+  Qed.
+      
+  Lemma extend_path'_preserves_uniq :
+    forall m p0 ps,
+      uniq_path_t p0 -> extend_path' m p0 = ps -> all (fun p => uniq_path_t p) ps.
+  Proof.
+    intros. subst ps. unfold extend_path'.
+    rewrite all_map. simpl.
+    unfold preim. simpl.
+    apply/allP.
+    intros. simpl. unfold uniq_path_t. rewrite cons_uniq. simpl. unfold uniq_path_t in H.
+    rewrite cons_uniq in H.
+    rewrite mem_filter in H0.
+    apply/and3P.
+    pose (Hprop := andb_prop _ _ H).
+    destruct Hprop as [G1 G2].
+    split; auto.
+    Admitted.
+    
+  
   Definition path := (seq (Component.id * Block.id)).
   SearchAbout seq.
 
@@ -309,18 +355,23 @@ Module Memory.
 
   Definition component_memories_of_memory (m: t) : seq ComponentMemory.t :=
     map snd (elementsm m).
+  
+  Definition list_of_per_component_set_of_block_ids (m: t) : seq {fset Block.id} :=
+    map ComponentMemory.domm (component_memories_of_memory m).
+  
+  (* I expect that the use of "val" that converts a set to a sequence can be problematic
+     because there aren't really useful lemmas about size and val.
+     
+     However, I don't know for now how to "map size" to a seq of "fset"s.
 
-  Definition all_block_ids_of_memory (m: t) : {fset Block.id} :=
-    fold_left fsetU (map ComponentMemory.domm(component_memories_of_memory m)) fset0.
+     I do not even know if the seq that val returns contains any duplicates.
+     I assume it doesn't.
+   *)
+  Definition count_of_allocated_blocks_of_memory (m: t) : nat :=
+    sumn (map (fun x => size (val x)) (list_of_per_component_set_of_block_ids m)).
 
-  Definition number_of_allocated_blocks_of_memory (m: t) : nat :=
-    size (all_block_ids_of_memory m).
-
-
-  (* This definition is wrong. Instead need to properly count the blocks. Now we're counting 
-   the number of component memories.*)
   Definition reachable_paths (m: t) (bs: {fset path}) :=
-    reachable_paths_with_fuel m bs (number_of_allocated_blocks_of_memory m).
+    reachable_paths_with_fuel m bs (count_of_allocated_blocks_of_memory m).
 
   Check maxn.
   Check foldl.
@@ -421,7 +472,7 @@ Module Memory.
 
   SearchAbout seq.
   Lemma extend_path_never_produces_cycles :
-    forall m p lp,
+    forall m (p : path) lp,
       uniq p ->
       extend_path m p = lp ->
       all uniq lp.
